Update Refine, add results on pure ctrees

theories/Interp/Refine.v
@@ -14,51 +14,176 @@ Import ITree.Basics.Basics.Monads.
 Import MonadNotation.
 Open Scope monad_scope.
 
-Variant pureb {E C X} (rec : ctree E C X -> Prop) : ctree' E C X -> Prop :=
-  | pure_ret   (v : X) : pureb rec (RetF v)
-  | pure_delay {Y} (c: C Y) k (REC: forall v, rec (k v)) : pureb rec (BrDF c k).
+Variant pureb {E C X} (rec : ctree E C X -> Prop) (t : ctree E C X) : Prop :=
+  | pureb_ret   (v : X) (EQ : t ≅ Ret v) : pureb rec t
+  | pureb_delay {Y} (c: C Y) k (EQ : t ≅ BrD c k) (REC: forall v, rec (k v)) : pureb rec t.
 
-Definition pureb_ {E C X} rec (t : ctree E C X) := pureb rec (observe t).
-
-Program Definition fpure {E C R} : mon (ctree E C R -> Prop) := {|body := pureb_|}.
+Program Definition fpure {E C R} : mon (ctree E C R -> Prop) := {|body := pureb|}.
 Next Obligation.
-  red in H0 |- *.
-  inversion_clear H0; econstructor; auto.
+  inversion_clear H0; [eleft | eright]; eauto.
 Qed.
 
-Definition pure {E C R} := gfp (@fpure E C R).
+Section pure.
 
-Inductive pure_finite {E C X} : ctree E C X -> Prop :=
-  | puref_ret (v : X) : pure_finite (Ret v)
-  | puref_delay {Y} (c: C Y) (k : Y -> ctree E C X) (REC: forall v, pure_finite (k v)) : pure_finite (BrD c k).
+  Context {E C : Type -> Type} {X : Type}.
+
+  Class pure (t : ctree E C X) := pure_ : gfp (@fpure E C X) t.
+
+  #[global] Instance pure_equ : Proper (@equ E C X X eq ==> flip impl) pure.
+  Proof.
+    cbn. intros. step in H0. inversion H0.
+    - step. eleft. now rewrite H, EQ.
+    - step. eright. now rewrite H, EQ. apply REC.
+  Qed.
+
+  #[global] Instance pure_ret r : pure (Ret r).
+  Proof.
+    step. now eleft.
+  Qed.
+
+  #[global] Instance pure_br {T} (c : C T) k :
+    (forall x, pure (k x)) ->
+    pure (BrD c k).
+  Proof.
+    intros. step. now eright.
+  Qed.
+
+  #[global] Instance pure_guard `{B1 -< C} t :
+    pure t ->
+    pure (Guard t).
+  Proof.
+    intros. unfold Guard. step. now eright.
+  Qed.
+
+  #[global] Instance pure_stuck `{B0 -< C} :
+    pure stuckD.
+  Proof.
+    unfold stuckD. step. now eright.
+  Qed.
+
+  Lemma trans_pure_is_val `{B0 -< C} (t t' : ctree E C X) l :
+    pure t ->
+    trans l t t' ->
+    is_val l.
+  Proof.
+    intros. do 3 red in H1. genobs t ot. genobs t' ot'.
+    assert (t ≅ go ot). { now rewrite Heqot, <- ctree_eta. } clear Heqot.
+    revert t H0 H2. induction H1; intros; subst.
+    - apply IHtrans_ with (t := k x); auto. 2: apply ctree_eta.
+      rewrite H2 in H0. step in H0. inversion H0; inv_equ.
+      rewrite EQ0. apply REC.
+    - rewrite H2 in H1. step in H1. inversion H1; inv_equ.
+    - rewrite H2 in H1. step in H1. inversion H1; inv_equ.
+    - constructor.
+  Qed.
+
+End pure.
+
+Section pure_finite.
+
+  Context {E C : Type -> Type} {X : Type}.
+
+  Inductive pure_finite_ : ctree E C X -> Prop :=
+    | puref_ret (v : X) t (EQ: t ≅ Ret v) : pure_finite_ t
+    | puref_delay {Y} (c: C Y) (k : Y -> ctree E C X) t (EQ: t ≅ BrD c k) (REC: forall v, pure_finite_ (k v)) : pure_finite_ t.
+
+  Class pure_finite (t : ctree E C X) : Prop :=
+    pure_finite__ : pure_finite_ t.
+
+  #[global] Instance pure_finite_equ :
+    Proper (equ eq ==> flip impl) pure_finite.
+  Proof.
+    cbn. intros. revert x H. induction H0; intros.
+    - eleft. now subs.
+    - eright. now subs.
+      intro. now eapply H.
+  Qed.
+
+  #[global] Instance pure_finite_ret r : pure_finite (Ret r).
+  Proof.
+    now eleft.
+  Qed.
+
+  #[global] Instance pure_finite_br {T} (c : C T) k :
+    (forall x, pure_finite (k x)) ->
+    pure_finite (BrD c k).
+  Proof.
+    now eright.
+  Qed.
+
+  #[global] Instance pure_finite_guard `{B1 -< C} t :
+    pure_finite t ->
+    pure_finite (Guard t).
+  Proof.
+    unfold Guard. now eright.
+  Qed.
+
+  #[global] Instance pure_finite_stuck `{B0 -< C} :
+    pure_finite stuckD.
+  Proof.
+    unfold stuckD. now eright.
+  Qed.
+
+End pure_finite.
+
+Lemma pure_finite_bind_R {E C X Y} :
+  forall R t (k : X -> ctree E C Y),
+  t (≅R) t ->
+  pure_finite t ->
+  (forall x, R x x -> pure_finite (k x)) ->
+  pure_finite (CTree.bind t k).
+Proof.
+  intros. induction H0.
+  - subs. inv_equ. rewrite bind_ret_l; auto.
+  - subs. inv_equ. rewrite bind_br. apply pure_finite_br. auto.
+Qed.
+
+#[global] Instance pure_finite_bind {E C X Y} :
+  forall t (k : X -> ctree E C Y),
+  pure_finite t ->
+  (forall x, pure_finite (k x)) ->
+  pure_finite (CTree.bind t k).
+Proof.
+  intros. apply (pure_finite_bind_R eq); auto.
+Qed.
+
+Lemma pure_pure_finite {E C X} :
+  forall (t : ctree E C X),
+  pure_finite t ->
+  pure t.
+Proof.
+  intros. induction H; subs; step.
+  - now eleft.
+  - now eright.
+Qed.
+
+Lemma is_stuck_pure : forall {E B X Y} `{B0 -< B} t (k : X -> ctree E B Y),
+  pure t ->
+  (forall x, is_stuck (k x)) ->
+  is_stuck (CTree.bind t k).
+Proof.
+  red. intros. intro.
+  apply trans_bind_inv in H2 as [].
+  - destruct H2 as (? & ? & ? & ?). subs.
+    apply H2. eapply trans_pure_is_val; eauto.
+  - destruct H2 as (? & ? & ?). now apply H1 in H3.
+Qed.
 
 Definition refine' {E C M : Type -> Type}
            {FM : Functor M} {MM : Monad M}
            {IM : MonadIter M} {FoM : MonadTrigger E M}
-           {CM : MonadBr B01 M}
+           {CM : MonadBr void1 M}
            (h : C ~> M) :
   ctree E (B01 +' C) ~> M :=
   refine (fun b X (c: (B01 +' C) X) =>
     match c, X return M X with
-    | inl1 c, X => mbr b c
-    | inr1 c, X => r <- h X c;; mbr b (inr1 branch1);; ret r
+    | inl1 c, X => mbr b (inl1 c)
+    | inr1 c, X => r <- h X c;; mbr b (inl1 (inr1 branch1));; ret r
     end).
-
-#[global] Instance MonadBr_subevent_l : forall {E B B'}, MonadBr B (ctree E (B +' B')).
-Proof.
-  red. intros. eapply MonadBr_ctree; eauto.
-  Unshelve. now left.
-Defined.
-#[global] Instance MonadBr_stateT_subevent_l : forall {E B B' St}, MonadBr B (stateT St (ctree E (B +' B'))).
-Proof.
-  typeclasses eauto.
-Defined.
 
 Definition refine'_state {E C D St} (f : C ~> stateT St (ctree E (B01 +' D))) :
   ctree E (B01 +' C) ~> stateT St (ctree E (B01 +' D)) :=
   refine' (CM := MonadBr_stateT) f.
-
-Unset Universe Checking.
 
 Import SSim'Notations.
 
@@ -68,11 +193,13 @@ Theorem ssim_pure {E F B C X} `{HasB0: B0 -< B} `{HasB0': B0 -< C} : forall (L :
   ssim L t (Ret tt : ctree F C unit).
 Proof.
   intros. induction H.
-  - now apply ssim_ret.
-  - now apply ssim_brD_l.
+  - subs. now apply ssim_ret.
+  - subs. now apply ssim_brD_l.
 Qed.
 
-Theorem refine_ctree_ssim {E B B' X} `{HasB0: B0 -< B'} `{HasB1: B1 -< B'} :
+Unset Universe Checking.
+
+Theorem refine_ctree_ssim {E B B' X} :
   forall (t : ctree E (B01 +' B) X) (h : B ~> ctree E (B01 +' B')),
   (forall X c, pure_finite (h X c)) ->
   refine' h _ t ≲ t.
@@ -85,7 +212,7 @@ Proof.
   - setoid_rewrite bind_trigger.
     apply step_ss'_vis_id. intros. split; [|auto].
     step. apply step_ss'_guard_l. apply CH.
-  - unfold mbr, MonadBr_subevent_l, MonadBr_ctree. destruct c.
+  - unfold mbr, MonadBr_ctree. destruct c.
     + setoid_rewrite bind_branch.
       apply step_ssbt'_br_id; auto. intros.
       step. apply step_ss'_guard_l. apply CH.
@@ -99,17 +226,10 @@ Proof.
       rewrite bind_ret_l. step. apply step_ss'_guard_l. apply CH.
 Qed.
 
-Variant lift_val_rel {E X Y} (R : rel X Y): @label E -> @label E -> Prop :=
-| Rel_Val (v1 : X) (v2 : Y) : R v1 v2 -> lift_val_rel R (val v1) (val v2)
-| Rel_Tau : lift_val_rel R tau tau
-| Rel_Obs : forall {X X'} e e' (x : X) (x' : X'), obs e x = obs e' x' -> lift_val_rel R (obs e x) (obs e' x')
-.
-#[global] Hint Constructors lift_val_rel : trans.
-
 Definition Rrr {St X} (p : St * X) (x : X) := snd p = x.
 Definition Lrr {St E X} := @lift_val_rel E _ X (@Rrr St X).
 
-Theorem refine_state_ssim {E B B' X St} `{HasB0: B0 -< B'} `{HasB1: B1 -< B'} :
+Theorem refine_state_ssim {E B B' X St} :
   forall (t : ctree E (B01 +' B) X) (h : B ~> stateT St (ctree E (B01 +' B'))),
   (forall X c s, pure_finite (h X c s)) ->
   forall s, refine' h _ t s (≲@Lrr St E X) t.
@@ -120,11 +240,11 @@ Proof.
   destruct (observe t) eqn:?.
   - apply step_ssbt'_ret. constructor. reflexivity.
   - setoid_rewrite bind_trigger.
-    rewrite bind_vis. apply step_ss'_vis_id. intros. split; [| constructor; auto].
+    rewrite bind_vis. apply step_ss'_vis_id. intros. split; [| constructor; etrans].
     step. rewrite bind_ret_l. apply step_ss'_guard_l. apply CH.
-  - unfold mbr, MonadBr_subevent_l, MonadBr_ctree. destruct c.
+  - unfold mbr, MonadBr_ctree. destruct c.
     + setoid_rewrite bind_branch. setoid_rewrite bind_br.
-      apply step_ssbt'_br_id; [| constructor]. intros.
+      apply step_ssbt'_br_id; [| constructor; etrans]. intros.
       step. setoid_rewrite bind_ret_l. apply step_ss'_guard_l. apply CH.
     + rewrite bind_bind.
       change (Br vis (inr1 b) k) with ((fun _ => Br vis (inr1 b) k) tt).
@@ -132,6 +252,6 @@ Proof.
       __upto_bind_ssim' (fun _ _ => True).
       { apply ssim_pure. apply H. intros. now constructor. }
       red. intros ? _ _. rewrite bind_bind, bind_branch, bind_br.
-      apply step_ssbt'_br; [| constructor]. intros ?. exists (snd x).
+      apply step_ssbt'_br; [| constructor; etrans]. intros ?. exists (snd x).
       rewrite bind_ret_l. step. rewrite bind_ret_l. apply step_ss'_guard_l. apply CH.
 Qed.
